src/lowparse/LowParse.Low.Int.fst
@@ -37,6 +37,15 @@ let parse32_u32 =
     Aux.parse32_u32 input
   )
 
+let serialize32_u8 = fun out lo v ->
+  let _ = Unique.serialize_u8_unique v in
+  Aux.serialize32_u8 out lo v;
+  let h = HST.get () in
+  let _ = Unique.parse_u8_unique (B.as_seq h (B.gsub out lo 1ul)) in
+  exactly_contains_valid_data_equiv h Aux.parse_u8 out lo v (U32.add lo 1ul);
+  exactly_contains_valid_data_equiv h parse_u8 out lo v (U32.add lo 1ul);
+  ()
+
 let serialize32_u16 = fun out lo v ->
   let _ = Unique.serialize_u16_unique v in
   Aux.serialize32_u16 out lo v;
@@ -54,6 +63,8 @@ let serialize32_u32 = fun out lo v ->
   exactly_contains_valid_data_equiv h Aux.parse_u32 out lo v (U32.add lo 4ul);
   exactly_contains_valid_data_equiv h parse_u32 out lo v (U32.add lo 4ul);
   ()
+
+let serialize32_u8_fail = serializer32_fail_of_serializer serialize32_u8 1l
 
 let serialize32_u16_fail = serializer32_fail_of_serializer serialize32_u16 2l
 
