src/lowparse/LowParse.SLow.Option.fst
@@ -1,25 +1,41 @@
 module LowParse.SLow.Option
-include LowParse.Spec.Option
+include LowParse.Low.Option
 include LowParse.SLow.Base
 
 module U32 = FStar.UInt32
 module B32 = FStar.Bytes
+module I32 = FStar.Int32
+module HST = FStar.HyperStack.ST
 
 inline_for_extraction
-let parse32_option (#k: parser_kind) (#t: Type) (#p: parser k t) (p32: parser32 p) : Tot (parser32 (parse_option p)) =
-  fun input -> ((match p32 input with
-  | Some (x, consumed) -> Some (Some x, consumed)
-  | _ -> Some (None, 0ul)) <: (y: option (option t * U32.t) { parser32_correct (parse_option p) input y } ))
+let parse32_option
+  (#k: parser_kind)
+  (#t: Type)
+  (#p: parser k t)
+  (v32: validator32 #default_validator32_cls p)
+  (p32: parser32 p)
+: Tot (parser32 (parse_option p))
+= fun input len ->
+  if v32 input len `I32.lt` 0l
+  then (None, 0l)
+  else
+    match p32 input len with
+    | (x, consumed) -> (Some x, consumed)
 
 inline_for_extraction
 let serialize32_option (#k: parser_kind) (#t: Type) (#p: parser k t) (#s: serializer p) (s32: serializer32 s) (u: squash (k.parser_kind_low > 0)) : Tot (serializer32 (serialize_option s u)) =
-  fun input -> ((match input with
+  fun output len lo input ->
+  match input with
   | None ->
-    [@inline_let]
-    let res = B32.empty_bytes in
-    assert (B32.reveal res `Seq.equal` Seq.empty);
-    res
-  | Some y -> s32 y) <: (y: B32.bytes { serializer32_correct (serialize_option s u) input y } ))
+    let h = HST.get () in
+    contains_valid_serialized_data_or_fail_equiv h (serialize_option s u) output lo None lo;
+    lo
+  | Some x ->
+    let hi = s32 output len lo x in
+    let h = HST.get () in
+    contains_valid_serialized_data_or_fail_equiv h s output lo x hi;
+    contains_valid_serialized_data_or_fail_equiv h (serialize_option s u) output lo (Some x) hi;
+    hi
 
 inline_for_extraction
 let size32_option (#k: parser_kind) (#t: Type) (#p: parser k t) (#s: serializer p) (s32: size32 s) (u: squash (k.parser_kind_low > 0)) : Tot (size32 (serialize_option s u)) =
