src/lowparse/LowParse.Low.Int.Aux2.fst
@@ -1,0 +1,11 @@
+module LowParse.Low.Int.Aux2
+
+module Seq = FStar.Seq
+
+let seq_equal_1
+  (#t: Type)
+  (s1 s2: Seq.seq t)
+: Lemma
+  (requires (Seq.length s1 == 1 /\ Seq.length s2 == 1 /\ Seq.index s1 0 == Seq.index s2 0))
+  (ensures (s1 == s2))
+= assert (s1 `Seq.equal` s2)
